veric/base.v
@@ -19,40 +19,9 @@ Require Export compcert.cfrontend.Clight.
 Require Export EqNat.  (* do we need this? *)
 Require Export msl.Coqlib2.
 Require Export veric.coqlib4.
-Require Export sepcomp.Address.
-
+Require Export veric.Memory.
 Set Implicit Arguments.
 
-Require Export msl.eq_dec.
-Instance EqDec_ident: EqDec ident := ident_eq.
-
-Instance EqDec_byte: EqDec byte := Byte.eq_dec.
-
-Instance EqDec_type: EqDec type := type_eq.
-
-Instance EqDec_int64: EqDec int64 := Int64.eq_dec.
-Instance EqDec_float32: EqDec float32 := Float32.eq_dec.
-
-Instance EqDec_memval: EqDec memval.
-Proof.
-  hnf. repeat decide equality; apply eq_dec.
-Defined.
-
-Instance EqDec_val: EqDec val.
-Proof.
-hnf. decide equality; apply eq_dec.
-Defined.
-
-Instance EqDec_quantity: EqDec quantity.
-Proof.
-hnf. decide equality.
-Defined.
-
 Definition funsig := (list (ident*type) * type)%type. (* argument and result signature *)
-
-Lemma range_dec: forall a b c: Z, {a <= b < c}+{~(a <= b < c)}.
-Proof. intros. destruct (zle a b). destruct (zlt b c). left; split; auto.
-  right;  omega. right; omega.
-Qed.
 
 (*Open Scope Z.*)
