veric/compcert_rmaps.v
@@ -979,3 +979,24 @@ apply writable_readable; auto.
 Qed.
 
 Hint Resolve bytes_writable_readable : mem.
+
+Lemma rmap_age_i:
+ forall w w' : rmap,
+    level w = S (level w') ->
+   (forall l, resource_fmap (approx (level w')) (w @ l) = w' @ l) -> 
+    age w w'.
+Proof.
+intros.
+hnf.
+destruct (levelS_age1 _ _ H).
+assert (x=w'); [ | subst; auto].
+assert (level x = level w')
+  by (apply age_level in H1; omega).
+apply rmap_ext; auto.
+intros.
+specialize (H0 l).
+rewrite (age1_resource_at w x H1 l (w@l)).
+rewrite H2.
+apply H0.
+symmetry; apply resource_at_approx.
+Qed.
