veric/semax_call.v
@@ -1263,27 +1263,6 @@ unfold age1; simpl.
 apply age1_juicy_mem_unpack'; auto.
 Qed. (* maybe don't need this? *)
 
-Lemma rmap_age_i:
- forall w w' : rmap,
-    level w = S (level w') ->
-   (forall l, resource_fmap (approx (level w')) (w @ l) = w' @ l) -> 
-    age w w'.
-Proof.
-intros.
-hnf.
-destruct (levelS_age1 _ _ H).
-assert (x=w'); [ | subst; auto].
-assert (level x = level w')
-  by (apply age_level in H1; omega).
-apply rmap_ext; auto.
-intros.
-specialize (H0 l).
-rewrite (age1_resource_at w x H1 l (w@l)).
-rewrite H2.
-apply H0.
-symmetry; apply resource_at_approx.
-Qed.
-
 Lemma free_juicy_mem_resource_decay:
   forall jm b lo hi m' jm'
      (H : free (m_dry jm) b lo hi = Some m')
